working on CCAS

examples/CCAS.v
@@ -26,6 +26,983 @@ Class HasBeq (t : Type) := {
   beq_false : forall x y, beq x y = false -> x <> y;
 }.
 
+Module CASTaskImpl.
+  Import LinCCALBase.
+  Import LTSSpec.
+  Import Lang.
+  Import Semantics.
+  Import AssertionsSet.
+  Import RGILogic.
+  Import TPSimulation.
+  Import AtomicLTS CAS'Spec FAISpec CASTaskSpec.
+  Import (coercions, canonicals, notations) Sig.
+  Import (notations) LinCCAL.
+  Import (canonicals) Sig.Plus.
+  Open Scope prog_scope.
+  Open Scope rg_relation_scope.
+
+  Context (Val : Type).
+  Context (vInit : Val).
+
+  Definition E : layer_interface :=
+  {|
+    li_sig := Sig.Plus.omap (ECAS' ((CASTask Val) + Val)) EFAI;
+    li_lts := tens_lts VCAS' VFAI;
+    li_init := pair (Idle (inr vInit)) (Idle O);
+  |}.
+  
+  Definition F : layer_interface :=
+  {|
+    li_sig := ECASTask Val;
+    li_lts := VCASTask;
+    li_init := Idle (cts (inr vInit) O nil);
+  |}.
+
+  Definition allocTask_impl (_ : tid) : Prog (li_sig E) nat :=
+    inr fai >= i => Ret i.
+  
+  Definition tryPlaceTask_impl o n i (cid : tid) : Prog (li_sig E) ((CASTask Val) + Val) :=
+    inl (cas (inr o) (inl (CTask cid o n i))) >= r => Ret r.
+  
+  Definition tryResolveTask_impl tsk v (_ : tid) : Prog (li_sig E) unit :=
+    inl (cas (inl tsk) (inr v)) >= _ => Ret tt.
+End CASTaskImpl.
+
+
+Module CCASImpl.
+  Import LinCCALBase.
+  Import LTSSpec.
+  Import Lang.
+  Import Semantics.
+  Import AssertionsSet.
+  Import RGILogic.
+  Import TPSimulation.
+  Import AtomicLTS Reg'Spec CASTaskSpec CCASSpec.
+  Import (coercions, canonicals, notations) Sig.
+  Import (notations) LinCCAL.
+  Import (canonicals) Sig.Plus.
+  Open Scope prog_scope.
+  Open Scope rg_relation_scope.
+
+  Context (Val : Type).
+  Context (vInit : Val).
+  Context `{HasBeq Val}.
+
+  Definition E : layer_interface :=
+  {|
+    li_sig := Sig.Plus.omap (ECASTask Val) (EReg bool);
+    li_lts := tens_lts VCASTask VReg;
+    li_init := pair (Idle (cts (inr vInit) O nil)) (Idle true);
+  |}.
+  
+  Definition F : layer_interface :=
+  {|
+    li_sig := ECCAS Val;
+    li_lts := VCCAS;
+    li_init := Idle (pair vInit false);
+  |}.
+
+  (*
+    (* The current thread try to complete its task *)
+    (* I //\\ task_placed t o n *)
+    t: complete t o n
+    (* I //\\ alin t (linr ccas r)) *)
+
+    (* The current thread try to help other's task *)
+    (* I //\\ task_placed t' o n //\\ alin t (inv ccas) *)
+    t: complete t' o n
+    (* I //\\ alin t (inv ccas) *)
+  *)
+
+  Definition complete t o n i : Prog (li_sig E) unit :=
+    (* I //\\ (task_placed t o n i \\//
+        (cas !↦ task t o n i //\\
+            ((t = cid //\\ alin t (linr cas o))
+            \\// t <> cid)
+        )) *)
+    inr Reg'Spec.get >= b =>
+    (* I //\\
+            (* if cas succeed and b = true, resolve to (n, b, t ↦ linr cass o) *)
+            ((b = true //\\ task_succ t o n i)
+            (* if cas succeed and b = false, resolve to (o, b, t ↦ linr cass o) *)
+        \\// (b = false //\\ task_fail t o n i)
+            (* if cas failed, take this branch *)
+        \\// (cas !↦ task t o n i //\\
+                ((t = cid //\\ alin t (linr cas o))
+                \\// t <> cid)
+             ))
+    *)
+    inl (tryResolveTask (CTask t o n i)
+                        (match b with
+                          | true => n
+                          | false => o end)) >= _ =>
+    (* I //\\
+          ((t = cid //\\ alin t (linr cas o))
+          \\// t <> cid))
+    *)
+    Ret tt.
+  
+  (* 
+  task_placed t o n <=>
+          (* initial state *)
+          (cas ↦ task t o n //\\
+            ∃ b, { (o, b, t ↦ inv ccas) } ⊆ Δ ) \\//
+          (* right after linearize (b = true) *)
+          (cas ↦ task t o n //\\
+            (* { (o, true, t ↦ inv ccas), (n, true, t ↦ linr cass o) } ⊆ Δ ) \\// *)
+            ∃ b, { (o, b, t ↦ inv ccas), (n, b, t ↦ linr cass o) } ⊆ Δ ) \\//
+          (* right after linearize (b = false) *)
+          (cas ↦ task t o n //\\
+            (* { (o, false, t ↦ inv ccas), (o, false, t ↦ linr cass o) } ⊆ Δ ) \\// *)
+            ∃ b, { (o, b, t ↦ inv ccas), (o, b, t ↦ linr cass o) } ⊆ Δ ) \\//
+  *)
+
+  (* 
+  task_placed t o n i <=>
+        cas ↦ task t o n i //\\
+          ∃ b,
+          (* initial state *)
+            { (o, b, t ↦ inv ccas) } ⊆ Δ \\//
+          (* right after linearize (b = true) *)
+            { (o, b, t ↦ inv ccas), (n, b, t ↦ linr cass o) } ⊆ Δ \\//
+          (* right after linearize (b = false) *)
+            { (o, b, t ↦ inv ccas), (o, b, t ↦ linr cass o) } ⊆ Δ \\//
+          (* after interference *)
+            { (o, b, t ↦ inv ccas), (n, b, t ↦ linr cass o), (o, b, t ↦ linr cass o) } ⊆ Δ
+  *)
+
+  (* 
+  task_resolved cid t o n i <=>
+        cas !↦ task t o n i //\\
+            ((t = cid //\\ alin t (linr cas o))
+            \\// t <> cid)
+  *)
+        
+  (* 
+  task_succ t o n i <=>
+        cas ↦ task t o n i //\\
+          ∃ b,
+          (* right after linearize (b = true) *)
+            { (o, b, t ↦ inv ccas), (n, b, t ↦ linr cass o) } ⊆ Δ \\//
+          (* after interference *)
+            { (o, b, t ↦ inv ccas), (n, b, t ↦ linr cass o), (o, b, t ↦ linr cass o) } ⊆ Δ
+  *)
+
+  (* 
+  task_fail t o n i <=>
+        cas ↦ task t o n i //\\
+          ∃ b,
+          (* right after linearize (b = false) *)
+            { (o, b, t ↦ inv ccas), (o, b, t ↦ linr cass o) } ⊆ Δ \\//
+          (* after interference *)
+            { (o, b, t ↦ inv ccas), (n, b, t ↦ linr cass o), (o, b, t ↦ linr cass o) } ⊆ Δ
+  *)
+
+  Definition ccas_impl o n (cid : tid) : Prog (li_sig E) Val :=
+    inl (allocTask o n) >= i =>
+    Do {
+      (* I //\\ alin t (inv ccas) *)
+      inl (tryPlaceTask o n i) >= r =>
+      (* I //\\ 
+            (* failed *)
+            (r <> o //\\ isVal r //\\ alin t (linr ccas r))
+            (* other task *)
+            (r <> o //\\ alin t (inv ccas) //\\ r = task t' o' n' i' //\\ 
+                (task_placed t' o' n' i' \\// task_resolved t t' o' n' i'))
+            (* my task *)
+            (r = o //\\ task_placed t o n i)
+      *)
+      match r with
+      (* I //\\
+            (r <> o //\\ alin t (inv ccas) //\\ r = task t' o' n' i' //\\ 
+                (task_placed t' o' n' i' \\// task_resolved t t' o' n' i'))
+      *)
+      | inl (CTask t o n i) =>
+          (complete t o n i) ;;
+          (* I //\\ r = task t' o' n' i' //\\ alin t (inv ccas) *)
+          Ret r
+      (* I //\\ 
+            (* failed *)
+            (r <> o //\\ isVal r //\\ alin t (linr ccas r))
+            (* my task *)
+            (r = o //\\ task_placed t o n)
+      *)
+      | _ => Ret r
+      end
+    } Loop >= r =>
+    (if beq r o then
+      (* I //\\ 
+            (r = o //\\ task_placed t o n)
+      *)
+      complete cid o n i
+      (* I //\\ 
+            (r = o //\\ alin t (linr ccas r))
+      *)
+    else
+      (* I //\\
+            (r <> o //\\ isVal r //\\ alin t (linr ccas r))
+      *)
+      Ret tt) ;;
+    Ret r.
+  
+  Definition setFlag_impl b (_ : tid) : Prog (li_sig E) unit :=
+    inr (set b) >= _ => Ret tt.
+
+  Definition assertion := @Assertion (@ProofState _ _ (li_lts E) (li_lts F)).
+  Definition rg_relation := @RGRelation _ _ (li_lts E) (li_lts F).
+
+  Open Scope rg_relation_scope.
+  Open Scope assertion_scope.
+
+  Instance PSS_Join_equiv : Join (@ProofState _ _ (li_lts E) (li_lts F)) :=
+    (@PSS_Join _ _ _ _ equiv_Join equiv_Join).
+
+  (* Task placed but not executed *)
+  Definition notDone t (o n : Val) : assertion :=
+    ALin' t (ls_inv (cas o n)) * (∃ b, (@Aρ _ _ _ (li_lts F) (Idle (pair o b)))).
+  
+  (* Task executed and succeeded *)
+  Definition endSucc t o n : assertion :=
+    ALin' t (ls_linr (cas o n) o) * (∃ b, @Aρ _ _ _ (li_lts F) (Idle (pair n b))).
+
+  (* Task executed but failed *)
+  Definition endFail t o n : assertion :=
+    ALin' t (ls_linr (cas o n) o) * (∃ b, @Aρ _ _ _ (li_lts F) (Idle (pair o b))).
+
+  Definition trySucc t o n : assertion :=
+    notDone t o n ⨁ endSucc t o n.
+  Definition tryFail t o n : assertion :=
+    notDone t o n ⨁ endFail t o n.
+  Definition tryBoth t o n : assertion :=
+    notDone t o n ⨁ endSucc t o n ⨁ endFail t o n.
+
+  Definition ACAS P : assertion := fun s => P (fst (σ s)).
+  Notation "'cas' ↦ v" :=
+    (ACAS (fun c => state c = v))
+    (at level 30, no associativity).
+  
+  Definition CTask t o n : assertion :=
+    cas ↦ inl (task t o n) //\\
+    (notDone t o n \\// trySucc t o n \\// tryFail t o n \\// tryBoth t o n).
+  Definition CVal : assertion :=
+    ∃ v : Val, cas ↦ inr v //\\ ∃ b, @Aρ _ _ _ (li_lts F) (Idle (pair v b)).
+  
+  Definition ICAS : assertion :=
+    CVal \\// ∃ t, ∃ o, ∃ n, CTask t o n.
+
+  Definition AFlag P : assertion := fun s => P (snd (σ s)).
+  Notation "'flag' ↦ v" :=
+    (AFlag (fun b => state b = v))
+    (at level 30, no associativity).
+  
+  Definition IFlag : assertion :=
+    ∃ b, flag ↦ b //\\ (fun s => forall ρ π, Δ s ρ π -> snd (state ρ) = b).
+    (* FIXME: the assertion below cannot handle the case with multiple possibilities *)
+    (* separation of v and b is necessary *)
+    (* ∃ v, @Aρ _ _ _ (li_lts F) (Idle (pair v b)). *)
+
+  (* MARK: for the sake of simplicity, use race-free register *)
+  (* Definition IRacy : assertion :=
+    ∀ t, ∀ b', ∀ s, AFlag (fun b => b = Pending s t (set b'))
+      ==>> (ALin' t (ls_inv (setFlag b'))). *)
+
+  Definition I : assertion := Inv.
+
+    (fun s => state (σ s) )
+            ((state (σ s) = None /\
+              exists ρt ρf, (Aρ ρt ⊕ Aρ ρf) s /\ state ρt = true /\ state ρf = false)
+            \/ (exists b, state (σ s) = Some b /\
+              exists ρ, Aρ ρ s /\ state ρ = b))
+        /\  (forall v t w, σ s = Pending v t (set w) ->
+              exists b : bool, @Aρ _ _ _ (li_lts F) (Pending b t flip) s)
+        /\  ((forall v w t, σ s <> Pending v t (set w)) -> exists b, @Aρ _ _ _ (li_lts F) (Idle b) s).
+    
+  
+  (* Definition I : assertion :=
+    fun s =>
+            (* state correspondence *)
+            ((state (σ s) = None /\ forall b, exists ρ π, Δ s ρ π /\ state ρ = b) \/
+            (exists b, state (σ s) = Some b /\ exists ρ π, Δ s ρ π /\ state ρ = b))
+            (* racy set implies racy flip *)
+        /\  (forall v t w, σ s = Pending v t (set w) ->
+              exists ρ π, Δ s ρ π /\ exists b, ρ = Pending b t flip)
+        /\  ((forall v w t, σ s <> Pending v t (set w)) -> forall ρ π, Δ s ρ π -> exists b, ρ = Idle b)
+        . *)
+  
+  Lemma idle_not_pending : forall (u v w : option bool) t, Idle u <> Pending v t (set w).
+  Proof. inversion 1. Qed.
+
+  Definition π_independent (P : assertion) := forall s1 s2,
+    σ s1 = σ s2 ->
+    (forall ρ1 π1, Δ s1 ρ1 π1 -> exists ρ2 π2, Δ s2 ρ2 π2 /\ ρ1 = ρ2) ->
+    (forall ρ2 π2, Δ s2 ρ2 π2 -> exists ρ1 π1, Δ s1 ρ1 π1 /\ ρ1 = ρ2) ->
+    P s1 -> P s2.
+
+  (* Lemma I_π_independent: π_independent I.
+  Proof.
+    unfold π_independent; intros.
+    unfold I in *. rewrite H in *.
+    destruct H2 as [? ?].
+    split; [|split].
+    - destruct H2.
+      + left.
+        destruct H2.
+        split; auto.
+        intros. specialize (H4 b) as [? [? [? ?]]].
+        specialize (H0 _ _ H4) as [? [? [? ?]]]; subst.
+        eauto.
+      + right.
+        destruct H2 as [b [? [? [? [? ?]]]]].
+        specialize (H0 _ _ H4) as [? [? [? ?]]]; subst.
+        eexists; eauto.
+    - intros.
+      eapply H3 in H4 as [? [? [? ?]]].
+      specialize (H0 _ _ H4) as [? [? [? ?]]]; subst.
+      eauto.
+    - destruct H3. intros.
+      apply H1 in H6 as [? [? [? ?]]]; subst.
+      eapply H4; eauto.
+  Qed. *)
+  
+
+  Definition domexact_G t : rg_relation := 
+    fun s1 s2 => forall t', t <> t' ->
+        forall ρ1 π1 ρ2 π2, Δ s1 ρ1 π1 -> Δ s2 ρ2 π2 -> TMap.find t' π1 = None <-> TMap.find t' π2 = None.
+  
+  Definition domexact_R t : rg_relation :=
+    fun s1 s2 =>
+      forall ρ1 π1 ρ2 π2, Δ s1 ρ1 π1 -> Δ s2 ρ2 π2 -> TMap.find t π1 = None <-> TMap.find t π2 = None.
+  
+  Lemma domexact_RG_compatible : forall t1 t2, t1 <> t2 -> (domexact_G t1 ⊆ domexact_R t2)%RGRelation.
+  Proof.
+    intros. intros ? ?.
+    unfold domexact_R, domexact_G.
+    intros. eapply H0; eauto.
+  Qed.
+
+  Lemma GINV_domexact : forall t1 t2, t1 <> t2 -> (GINV t1 ⊆ domexact_R t2)%RGRelation.
+  Proof.
+    intros. intros ? ?.
+    unfold domexact_R, GINV, Ginv, LiftRelation_Δ.
+    intros.
+    destruct H0 as [? [? [? ?]]].
+    apply H4 in H2.
+    inversion H2; subst.
+    rewrite PositiveMap.gso; auto.
+    eapply (ac_domexact (Δ x)); eauto.
+  Qed.
+
+  Lemma GRET_domexact : forall t1 t2, t1 <> t2 -> (GRET t1 ⊆ domexact_R t2)%RGRelation.
+  Proof.
+    intros. intros ? ?.
+    unfold domexact_R, GRET, Gret, LiftRelation_Δ.
+    intros.
+    destruct H0 as [? [? [? [? ?]]]].
+    apply H4 in H2.
+    inversion H2; subst.
+    rewrite PositiveMap.gro; auto.
+    eapply (ac_domexact (Δ x)); eauto.
+  Qed.
+
+  Lemma domexact_R_refl : forall t s, domexact_R t s s.
+  Proof.
+    intros. intros ? ?.
+    unfold domexact_R, GId.
+    intros; subst.
+    eapply (ac_domexact (Δ s)); eauto.
+  Qed.
+
+  Definition G t : rg_relation := domexact_G t ∩
+    fun s1 s2 => forall t' ls, t <> t' -> ALin t' ls s1 -> ALin t' ls s2.
+
+  Definition R t : rg_relation := domexact_R t ∩
+    fun s1 s2 => forall ls, ALin t ls s1 -> ALin t ls s2.
+
+  Lemma Istable {t} : Stable (R t) I I.
+  Proof. unfold Stable. apply ConjRightImpl, ImplRefl. Qed.
+
+  Lemma ALinstable {t ls}: Stable (R t) I (ALin t ls).
+  Proof.
+    unfold Stable, R.
+    intros ? [[? [? [? ?]]] ?] ? ? ?.
+    apply H1 in H. apply H in H3. auto.
+  Qed.
+
+  Lemma ALin'stable {t ls}: Stable (R t) I (ALin' t ls).
+  Proof.
+    unfold Stable, R.
+    intros ? [[? [? [? ?]]] ?] ? ? ?.
+    apply H1 in H. apply H in H3. auto.
+  Qed.
+
+  Create HintDb stableDB.
+  Hint Resolve Istable ALinstable : stableDB.
+
+  Program Definition Mcoin : layer_implementation E F := {|
+    li_impl m :=
+      match m with
+      | flip => flip_impl
+      | read => read_impl
+      end
+  |}.
+  Next Obligation.
+  eapply RGILogic.soundness with (R:=R) (G:=G) (I:=I).
+    (* valid RG *)
+    {
+      constructor.
+      unfold R. intros.
+      destruct H.
+      split; intros.
+      - pose proof ac_nonempty (Δ s) as [? [? ?]].
+        specialize (H2 _ _ H4).
+        specialize (H _ _ _ _ H4 H3).
+        rewrite <- H; auto.
+      - pose proof ac_nonempty (Δ s') as [? [? ?]].
+        specialize (H2 _ _ H4).
+        specialize (H _ _ _ _ H3 H4).
+        rewrite H; auto.
+    }
+    (* G ⊆ R *)
+    {
+      unfold G, R.
+      intros. intros ? ? ?.
+      destruct H0.
+      - destruct H0.
+        eapply domexact_RG_compatible in H0; eauto.
+        split; auto.
+      - do 2 destruct H0.
+        + split; [eapply GINV_domexact|]; eauto.
+          unfold GINV, Ginv, LiftRelation_Δ, ALin in *.
+          destruct H0 as [? [? [? ?]]].
+          intros. apply H2 in H4.
+          inversion H4; subst.
+          rewrite PositiveMap.gso; auto.
+          eapply H3; eauto.
+        + split; [eapply GRET_domexact|]; eauto.
+          unfold GRET, Gret, LiftRelation_Δ, ALin in *.
+          destruct H0 as [? [? [? [? ?]]]].
+          intros. apply H2 in H4.
+          inversion H4; subst.
+          rewrite PositiveMap.gro; auto.
+          eapply H3; eauto.
+        + split; auto.
+          apply domexact_R_refl.
+    }
+    (* method provable *)
+    {
+      intros t.
+      destruct f.
+      (* flip *)
+      {
+        (* precondition *)
+        exists (I //\\ ALin t (Semantics.ls_inv flip)).
+        (* postcondition *)
+        exists (fun ret => I //\\ ALin t (Semantics.ls_linr flip ret)).
+        constructor;
+        try solve_conj_impl;
+        try solve_conj_stable stableDB.
+        {
+          intros ? [? [? [? [? ?]]]].
+          split; auto.
+          - eapply I_π_independent; eauto.
+            intros.
+            exists ρ1. eexists; split; auto.
+            apply H2. constructor; eauto.
+            intros.
+            apply H2 in H3. inversion H3; subst.
+            exists ρ2. eexists; split; eauto.
+          - intros ? ? ?.
+            apply H2 in H3.
+            inversion H3; subst.
+            rewrite PositiveMap.gss; auto.
+        }
+        {
+          intros. intros [? [[? ?] [? [? ?]]]].
+          eapply I_π_independent; eauto.
+          intros. exists ρ1. eexists; split; auto.
+          apply H3. constructor; eauto.
+          intros.
+          apply H3 in H4. inversion H4; subst.
+          do 2 eexists; split; eauto.
+        }
+        {
+          intros.
+          destruct H.
+          unfold ALin in *.
+          eapply H1. eauto.
+        }
+        {
+          simpl; unfold flip_impl.
+          (* perror *)
+          eapply provable_perror with
+            (P' := I //\\ ALin t (ls_inv flip) //\\ fun s => forall v t' w, t <> t' -> σ s <> Pending v t' (set w)).
+          {
+            intros ? ?.
+            destruct (σ s) eqn:eq.
+            - left. split; eauto.
+              rewrite eq. congruence.
+            - destruct op;
+              try (left; split; eauto;
+              rewrite eq; congruence).
+              destruct (Pos.eq_dec t0 t).
+              + left. split; eauto. rewrite eq,e. congruence.
+              + right.
+                destruct H as [[_ ?] ?].
+                apply H in eq as [? [? [? [? ?]]]]; subst.
+                pose proof H1.
+                apply H0 in H1.
+                econstructor; eauto.
+                do 2 econstructor; eauto.
+                econstructor; eauto.
+          }
+          (* set *)
+          eapply provable_vis_safe with
+            (P' := I //\\ ALin t (ls_lini flip))
+            (Q' := fun _ => I //\\ ALin t (ls_linr flip tt));
+          try solve_conj_impl;
+          try solve_conj_stable stableDB.
+          (* no error *)
+          {
+            intros ? [[[_ ?] ?] ?].
+            intros ?.
+            inversion H2; subst.
+            dependent destruction H6.
+            specialize (H1 v t' w H4). auto.
+          }
+          (* inv *)
+          {
+              pupdate_intros_atomic.
+              dependent destruction Hstep0.
+              destruct Hpre as [[? ?] ?].
+              destruct H as [? [? ?]]. simpl in *.
+              specialize (H3 (idle_not_pending _)). clear H2.
+              destruct H.
+              (* two poss *)
+              {
+                destruct H as [? ?].
+                pose proof (H2 true) as [ρt [πt [Hposst ?]]].
+                pose proof (H2 false) as [ρf [πf [Hpossf ?]]].
+                clear H2.
+
+                pose proof H3 _ _ Hposst as [? ?]; subst.
+                pose proof H3 _ _ Hpossf as [? ?]; subst.
+                simpl in *; subst.
+                pose proof H0 _ _ Hposst.
+                pose proof H0 _ _ Hpossf.
+
+                pupdate_start.
+
+                pupdate_trylin_from Hposst.
+                pupdate_forward t0 (InvEv flip).
+                pupdate_finish.
+
+                eapply ACTrylinContinue.
+
+                pupdate_trylin_from Hpossf.
+                pupdate_forward t0 (InvEv flip).
+                pupdate_finish.
+
+                eapply ACTrylinFinish.
+
+                do 2 split.
+                - split; [|split]; simpl; auto.
+                  + left. split; auto. intros.
+                    destruct b;
+                    [ exists (Pending true t0 flip) | exists (Pending false t0 flip) ];
+                    eexists; split; auto;
+                    [ right | left ]; econstructor; eauto;
+                    do 2 constructor; try (do 2 econstructor); auto.
+                  + inversion 1; subst.
+                    do 2 eexists. split.
+                    * left. constructor; eauto.
+                      do 2 constructor; try (do 2 econstructor); auto.
+                    * eauto.
+                  + intros. exfalso. eapply H4. eauto.
+                - unfold ALin; simpl.
+                  inversion 1; subst;
+                  inversion H5; subst;
+                  rewrite PositiveMap.gss; auto.
+                - unfold domexact_G; intros; simpl in *.
+                  do 2 dependent destruction H6;
+                  rewrite PositiveMap.gso; auto;
+                  eapply (ac_domexact Δ1); eauto.
+                - unfold ALin; simpl.
+                  intros.
+                  do 2 dependent destruction H6;
+                  rewrite PositiveMap.gso; auto;
+                  eapply H5; eauto.
+              }
+              (* single poss *)
+              {
+                destruct H as [? [? [ρ [π [Hposs ?]]]]]; subst.
+
+                pose proof H3 _ _ Hposs as [? ?]; subst.
+                pose proof H0 _ _ Hposs.
+                simpl in *.
+
+                pupdate_start.
+
+                pupdate_trylin_from Hposs.
+                pupdate_forward t0 (InvEv flip).
+                pupdate_finish.
+
+                eapply ACTrylinFinish.
+
+                do 2 split.
+                - split; [|split]; simpl; auto.
+                  + right. eexists; split; eauto.
+                    do 2 eexists; split.
+                    constructor; auto.
+                    do 2 constructor; try (do 2 econstructor); auto.
+                    auto.
+                  + inversion 1; subst.
+                    do 2 eexists; split.
+                    constructor; auto.
+                    do 2 constructor; try (do 2 econstructor); auto.
+                    eauto.
+                  + intros. exfalso. eapply H2; eauto.
+                - unfold ALin; simpl.
+                  inversion 1; subst.
+                  rewrite PositiveMap.gss; auto.
+                - unfold domexact_G; intros; simpl in *.
+                  dependent destruction H5.
+                  rewrite PositiveMap.gso; auto;
+                  eapply (ac_domexact Δ1); eauto.
+                - unfold ALin; simpl.
+                  intros.
+                  dependent destruction H5;
+                  rewrite PositiveMap.gso; auto.
+                  eapply H4; eauto.
+              }
+          }
+          (* res *)
+          {
+              pupdate_intros_atomic.
+              dependent destruction Hstep0.
+              destruct Hpre as [[? [? ?]] ?]. simpl in *.
+              clear H1.
+              specialize (H0 _ _ _ eq_refl) as [ρ [π [Hposs [b ?]]]]; subst.
+              pose proof H2 _ _ Hposs.
+
+              pupdate_start.
+
+              pupdate_trylin_from Hposs.
+              pupdate_forward t0 (ResEv flip tt).
+              pupdate_finish.
+
+              eapply ACTrylinContinue.
+
+              pupdate_trylin_from Hposs.
+              pupdate_forward t0 (ResEv flip tt).
+              pupdate_finish.
+
+              eapply ACTrylinFinish.
+
+              Unshelve.
+              2:{ exact true. }
+              2:{ exact false. }
+
+              do 2 split.
+              - split; [|split]; simpl; auto.
+                + left. split; auto. intros.
+                  destruct b0;
+                  [ exists (Idle true) | exists (Idle false) ];
+                  eexists; split; eauto;
+                  [ right | left ];
+                  constructor; eauto;
+                  do 2 constructor; try (do 2 econstructor); auto.
+                + inversion 1.
+                + intros.
+                  do 2 dependent destruction H3; eauto.
+              - unfold ALin; simpl.
+                intros.
+                do 2 dependent destruction H1;
+                rewrite PositiveMap.gss; auto.
+              - unfold domexact_G; intros; simpl in *.
+                do 2 dependent destruction H4;
+                rewrite PositiveMap.gso; auto;
+                eapply (ac_domexact Δ1); eauto.
+              - unfold ALin; simpl.
+                intros.
+                do 2 dependent destruction H4;
+                rewrite PositiveMap.gso; auto;
+                eapply H3; eauto.
+          }
+
+          (* return *)
+          intros.
+          eapply provable_ret_safe; destruct ret;
+          try solve_conj_impl;
+          try solve_conj_stable stableDB;
+          try apply ImplRefl.
+        }
+      }
+      (* read *)
+      {
+        (* precondition *)
+        exists (I //\\ ALin t (Semantics.ls_inv read)).
+        (* postcondition *)
+        exists (fun ret => I //\\ ALin t (Semantics.ls_linr read ret)).
+        constructor;
+        try solve_conj_impl;
+        try solve_conj_stable stableDB.
+        {
+          intros ? [? [? [? [? ?]]]].
+          split; auto.
+          - eapply I_π_independent; eauto.
+            intros.
+            exists ρ1. eexists; split; auto.
+            apply H2. constructor; eauto.
+            intros.
+            apply H2 in H3. inversion H3; subst.
+            exists ρ2. eexists; split; eauto.
+          - intros ? ? ?.
+            apply H2 in H3.
+            inversion H3; subst.
+            rewrite PositiveMap.gss; auto.
+        }
+        {
+          intros. intros [? [[? ?] [? [? ?]]]].
+          eapply I_π_independent; eauto.
+          intros. exists ρ1. eexists; split; auto.
+          apply H3. constructor; eauto.
+          intros.
+          apply H3 in H4. inversion H4; subst.
+          do 2 eexists; split; eauto.
+        }
+        {
+          intros.
+          destruct H.
+          unfold ALin in *.
+          eapply H1. eauto.
+        }
+        {
+          simpl; unfold read_impl.
+          (* loop *)
+          eapply provable_doloop;
+          try solve_conj_impl;
+          try solve_conj_stable stableDB.
+
+          (* get *)
+          eapply provable_vis_safe with
+            (P' := I //\\ ALin t (ls_inv read))
+            (
+              Q' := fun c =>
+                match c with
+                | Some b => I //\\ ALin t (ls_linr read b)
+                | None => I //\\ ALin t (ls_inv read)
+                end
+            );
+          try ((try destruct a); solve_conj_impl);
+          try ((try destruct a); solve_conj_stable stableDB).
+          (* no error *)
+          (* TODO: extract a more general tactic for solving no error *)
+          {
+            apply ImplTauto; intros ? H; destruct σ;
+            inversion H; subst.
+            dependent destruction H5.
+          }
+          (* inv *)
+          {
+            pupdate_intros_atomic.
+            dependent destruction Hstep0.
+            destruct Hpre as [[? [? ?]] ?]; simpl in *.
+
+            pupdate_start.
+            apply ac_steps_refl.
+
+            do 2 split; auto.
+            - split; [|split]; simpl; auto; try inversion 1.
+              intros. eapply H1; eauto.
+              apply idle_not_pending.
+            - unfold domexact_G. simpl. intros.
+              eapply (ac_domexact Δ1); eauto.
+          }
+          (* res *)
+          {
+            intro b.
+            pupdate_intros_atomic.
+            dependent destruction Hstep0.
+            destruct Hpre as [[? [? ?]] ?]; simpl in *.
+            (* clear H1 H0. *)
+            destruct H as [[? ?] | ?]; subst; simpl in *.
+            (* None *)
+            {
+              pupdate_start.
+              apply ac_steps_refl.
+
+              do 2 split; auto.
+              - split; [|split]; simpl; auto; try inversion 1; subst.
+                intros. eapply H1; eauto. inversion 1.
+              - unfold domexact_G. simpl. intros.
+                eapply (ac_domexact Δ1); eauto.
+            }
+            (* Some *)
+            {
+              destruct H as [b0 [? [ρ [π [Hposs ?]]]]]; subst. simpl in *.
+              clear H0.
+              pose proof Hposs.
+              eapply H1 in H as [? ?]; try congruence; subst; simpl in *.
+
+              pupdate_start.
+
+              pupdate_trylin_from Hposs.
+              pupdate_forward t0 (InvEv read).
+              pupdate_forward t0 (ResEv read x).
+              pupdate_finish.
+
+              apply ACTrylinFinish.
+
+              do 2 split.
+              - split; [|split]; simpl; auto.
+                + right. eexists; split; eauto.
+                  exists (Idle x); eexists; split; auto.
+                  econstructor; auto.
+                  apply H2 in Hposs.
+                  eapply rt_trans; do 2 constructor; auto;
+                  try constructor;
+                  [apply step_read_inv | apply step_read_res |].
+                  rewrite PositiveMap.gss; auto.
+                + inversion 1.
+                + intros. dependent destruction H0; eauto.
+              - unfold ALin; simpl.
+                intros. dependent destruction H.
+                rewrite PositiveMap.gss. auto.
+              - unfold domexact_G; simpl.
+                intros. dependent destruction H3.
+                do 2 try rewrite PositiveMap.gso; auto.
+                eapply (ac_domexact Δ1); eauto.
+              - unfold ALin; simpl.
+                intros. dependent destruction H3.
+                do 2 try rewrite PositiveMap.gso; eauto.
+            }
+          }
+
+          destruct ret; 
+          try (eapply provable_ret_safe;
+          try solve_conj_impl;
+          try solve_conj_stable stableDB;
+          try apply ImplRefl).
+
+          (* TODO: get the random value properly *)
+          (* cas *)
+          eapply provable_vis_safe with
+            (P' := I //\\ ALin t (ls_inv read))
+            (Q' := fun (succ : bool) => if succ then I //\\ ALin t (ls_linr read rand) else I //\\ ALin t (ls_inv read));
+          try ((try destruct a); solve_conj_impl);
+          try ((try destruct a); solve_conj_stable stableDB).
+          (* no error *)
+          {
+            apply ImplTauto; intros ? H; destruct σ;
+            inversion H; subst.
+            dependent destruction H5.
+          }
+          (* inv *)
+          {
+            pupdate_intros_atomic.
+            dependent destruction Hstep0.
+            destruct Hpre as [[? [? ?]] ?]; simpl in *.
+
+            pupdate_start.
+            apply ac_steps_refl.
+
+            do 2 split; auto.
+            - split; [|split]; simpl; auto; try inversion 1.
+              intros. eapply H1; eauto.
+              apply idle_not_pending.
+            - unfold domexact_G. simpl. intros.
+              eapply (ac_domexact Δ1); eauto.
+          }
+          (* res *)
+          {
+            intro b.
+            pupdate_intros_atomic.
+            destruct Hpre as [[? [? ?]] ?]; simpl in *.
+            remember (ResEv (cas None (Some rand)) b) as e in Hstep0.
+            inversion Hstep0; subst; try inversion H5; subst.
+            (* succ *)
+            {
+              clear H0.
+              apply ResEvInversion in H5; subst.
+              destruct H as [[_ ?] | [? [? ?]]]; [|congruence].
+              specialize (H rand) as [ρ [π [Hposs ?]]].
+              pose proof Hposs.
+              eapply H1 in H0 as [? ?]; subst; try congruence.
+              simpl in *; subst.
+              
+              pupdate_start.
+
+              pupdate_trylin_from Hposs.
+              pupdate_forward t0 (InvEv read).
+              pupdate_forward t0 (ResEv read rand).
+              pupdate_finish.
+
+              apply ACTrylinFinish.
+
+              do 2 split.
+              - split; [|split]; simpl.
+                + right. eexists; split; eauto.
+                  do 2 eexists; split; econstructor; auto.
+                  apply H2 in Hposs.
+                  eapply rt_trans; do 2 constructor; try do 2 constructor; auto.
+                  rewrite PositiveMap.gss; auto.
+                + congruence.
+                + intros.
+                  dependent destruction H0. eauto.
+              - unfold ALin; simpl.
+                intros. dependent destruction H.
+                rewrite PositiveMap.gss; auto.
+              - unfold domexact_G; simpl.
+                intros. dependent destruction H3.
+                do 2 (rewrite PositiveMap.gso; auto).
+                eapply (ac_domexact Δ1); eauto.
+              - unfold ALin; simpl. intros.
+                dependent destruction H3.
+                do 2 (rewrite PositiveMap.gso; eauto).
+            }
+            {
+              clear H0.
+              inversion H4; subst.
+              apply ResEvInversion in H4; subst.
+              destruct H as [[? ?] | [? [? [ρ [π [Hposs ?]]]]]]; try congruence; subst.
+              clear H8.
+              pose proof Hposs.
+              eapply H1 in H as [? ?]; subst; try congruence.
+
+              pupdate_start.
+              apply ac_steps_refl.
+              
+              do 2 split; auto.
+              - split; [|split]; simpl.
+                + right. eexists; split; eauto.
+                + congruence.
+                + intros. eapply H1; eauto.
+                  congruence.
+              - unfold domexact_G; simpl. intros.
+                eapply (ac_domexact Δ1); eauto.
+            }
+          }
+
+          (* return *)
+          destruct ret;
+          eapply provable_ret_safe;
+          try solve_conj_impl;
+          try solve_conj_stable stableDB;
+          try apply ImplRefl.
+        }
+      }
+    }
+    {
+      split; [|split]; simpl.
+      - right. eexists; split; eauto.
+        do 2 eexists; split; try constructor.
+      - congruence.
+      - intros. dependent destruction H0. eauto.
+    }
+  Defined.
+
+End CCASImpl.
+
 Module CCASImpl.
   Import LinCCALBase.
   Import LTSSpec.
@@ -61,17 +1038,17 @@ Module CCASImpl.
     li_init := Idle (pair vInit false);
   |}.
 
-(*
-  (* The current thread try to complete its task *)
-  (* I //\\ task_placed t o n *)
-  t: complete t o n
-  (* I //\\ alin t (linr ccas r)) *)
+  (*
+    (* The current thread try to complete its task *)
+    (* I //\\ task_placed t o n *)
+    t: complete t o n
+    (* I //\\ alin t (linr ccas r)) *)
 
-  (* The current thread try to help other's task *)
-  (* I //\\ task_placed t' o n //\\ alin t (inv ccas) *)
-  t: complete t' o n
-  (* I //\\ alin t (inv ccas) *)
-*)
+    (* The current thread try to help other's task *)
+    (* I //\\ task_placed t' o n //\\ alin t (inv ccas) *)
+    t: complete t' o n
+    (* I //\\ alin t (inv ccas) *)
+  *)
 
   Definition complete cid t o n i : Prog (li_sig E) unit :=
     (* I //\\ (task_placed t o n i \\//
@@ -131,7 +1108,7 @@ Module CCASImpl.
   *)
 
   (* 
-  task_cleared cid t o n i <=>
+  task_resolved cid t o n i <=>
         cas !↦ task t o n i //\\
             ((t = cid //\\ alin t (linr cas o))
             \\// t <> cid)
@@ -168,14 +1145,14 @@ Module CCASImpl.
             (r <> o //\\ isVal r //\\ alin t (linr ccas r))
             (* other task *)
             (r <> o //\\ alin t (inv ccas) //\\ r = task t' o' n' i' //\\ 
-                (task_placed t' o' n' i' \\// task_cleared t t' o' n' i'))
+                (task_placed t' o' n' i' \\// task_resolved t t' o' n' i'))
             (* my task *)
             (r = o //\\ task_placed t o n i)
       *)
       match r with
       (* I //\\
             (r <> o //\\ alin t (inv ccas) //\\ r = task t' o' n' i' //\\ 
-                (task_placed t' o' n' i' \\// task_cleared t t' o' n' i'))
+                (task_placed t' o' n' i' \\// task_resolved t t' o' n' i'))
       *)
       | inl (task t o n i) =>
           (complete cid t o n i) ;;
@@ -961,6 +1938,6 @@ Module CCASImpl.
     }
   Defined.
 
-End OneShotLazyCoinImpl.
+End CCASImpl.
 
 Print Assumptions OneShotLazyCoinImpl.Mcoin.
